src/Idempotent.v
@@ -1,13 +1,24 @@
 Require Import Hoare.
 Require Import Prog.
 Require Import Pred.
+Require Import SepAuto.
+Require Import Classical_Prop.
 
 Definition preserves_precondition (pre : pred) p :=
   forall m m' out, pre m -> exec m p m' out -> pre m' /\ out <> Failed.
 
-Theorem pp_add_lift : forall pre P p,
-  preserves_precondition pre p ->
-  preserves_precondition (pre * [[ P ]]) p.
+Theorem pp_exists : forall p T pre, (forall (x:T), preserves_precondition (pre x) p)
+  -> preserves_precondition (exists (x:T), pre x) p.
+Proof.
+  unfold preserves_precondition; intros.
+  destruct H0.
+  edestruct H; eauto.
+  split; eauto.
+  eexists; eauto.
+Qed.
+
+Theorem pp_add_lift : forall pre P p, preserves_precondition pre p
+  -> preserves_precondition (pre * [[ P ]]) p.
 Proof.
   unfold preserves_precondition; intros.
   apply sep_star_lift2and in H0; destruct H0.
@@ -17,10 +28,9 @@ Proof.
   split; eauto.
 Qed.
 
-Theorem pp_drop_lift : forall pre (P : Prop) p,
-  P ->
-  preserves_precondition (pre * [[ P ]]) p ->
-  preserves_precondition pre p.
+Theorem pp_drop_lift : forall pre (P : Prop) p, P
+  -> preserves_precondition (pre * [[ P ]]) p
+  -> preserves_precondition pre p.
 Proof.
   unfold preserves_precondition; intros.
   edestruct H0; clear H0; eauto.
@@ -29,11 +39,10 @@ Proof.
   eauto.
 Qed.
 
-Theorem idempotent_ok' : forall p p1 p2 pre,
-  preserves_precondition pre p ->
-  p1 = p ->
-  p2 = p ->
-  {{ pre }} p1 >> p2.
+Theorem idempotent_ok' : forall p p1 p2 pre, preserves_precondition pre p
+  -> p1 = Check pre ;; p
+  -> p2 = Check pre ;; p
+  -> {{ pre }} p1 >> p2.
 Proof.
   unfold corr at 1.
   intros.
@@ -42,79 +51,178 @@ Proof.
   | [ H: exec_recover _ _ _ _ _ |- _ ] => induction H; subst; auto
   end.
 
-  edestruct H; eauto; congruence.
-  apply IHexec_recover; auto.
-  edestruct H; eauto.
+  - inversion H3; subst.
+    edestruct H; eauto; congruence.
+    rewrite check_id_ok in *; congruence.
+  - inversion H3; subst; eauto.
+    edestruct H; eauto.
 Qed.
 
-Theorem idempotent_ok : forall p pre,
-  preserves_precondition pre p ->
-  {{ pre }} p >> p.
+Theorem idempotent_ok : forall p pre, preserves_precondition pre p
+  -> {{ pre }} Check pre ;; p >> Check pre ;; p.
 Proof.
   intros.
   eapply idempotent_ok'; eauto.
 Qed.
 
-(*
-Theorem corr_to_pp : forall p1 p2 pre1 pre2,
-  {{ pre1 }} p1 >> Check pre2 ;; p2 ->
-  (pre1 ==> [ pre2 ==> pre1 ]) ->
-  preserves_precondition pre1 p1.
+Theorem check_to_post : forall p1 p2 pre id, {{ pre }} p1 >> CheckID id ;; p2
+  -> forall m m' out, pre m -> exec m p1 m' out -> check_cond id m'.
+Proof.
+  unfold corr; intros.
+  destruct out.
+  - assert (Failed = Finished); eauto. discriminate.
+  - assert (exec m p1 m' Crashed) by (eapply prog_can_crash; eauto); clear H1.
+    assert (exists p, p = CheckID id ;; p2) as Hp by eauto. destruct Hp.
+    assert (exists p, p = CheckID id ;; p2) as Hp by eauto. destruct Hp.
+    destruct (exec_recover_can_terminate x x0 m').
+    destruct H4.
+    induction H4; subst.
+    + assert (Failed = Finished); eauto. discriminate.
+    + inversion H4; eauto.
+    + inversion H4; subst; eauto.
+  - assert (exists p, p = CheckID id ;; p2) as Hp by eauto. destruct Hp.
+    assert (exists p, p = CheckID id ;; p2) as Hp by eauto. destruct Hp.
+    destruct (exec_recover_can_terminate x x0 m').
+    destruct H4.
+    induction H4; subst.
+    + assert (Failed = Finished); eauto. discriminate.
+    + inversion H4; eauto.
+    + inversion H4; subst; eauto.
+Qed.
+
+Hint Resolve check_to_post.
+
+Theorem corr_to_pp : forall p1 p2 pre1 pre2id, {{ pre1 }} p1 >> CheckID pre2id ;; p2
+  -> (pre1 ==> pre1 * [[ check_cond pre2id ==> pre1 ]])
+  -> preserves_precondition pre1 p1.
 Proof.
   unfold preserves_precondition.
   intros.
   unfold corr in H.
+  apply H0 in H1 as Hcheck.
+  apply sep_star_lift2and in Hcheck.
+  unfold lift in *; destruct Hcheck.
   destruct out.
-  - exfalso.
-    destruct (H m RFailed); eauto.
-  - do 2 eexists; split; eauto.
-
-    assert (exec m p1 (Stopped m0 Crashed)) by ( eapply prog_can_crash; eauto ).
-    clear H2.
-
-    assert (forall out, exec m0 (Check pre2 ;; p2) out -> out <> Failed).
-    + unfold not in *; intros; subst; eauto.
-    + destruct (exec_need_not_crash (Check pre2 ;; p2) m0).
-      destruct H4.
-      inversion H4; subst.
-      * exfalso. edestruct H2; eauto.
-      * eapply H0; eauto.
+  - assert (Failed = Finished); [| discriminate ].
+    eapply H; eauto.
+  - split; try discriminate; eauto.
+  - split; try discriminate; eauto.
 Qed.
-*)
+
+Theorem corr_drop_check1 : forall pre p1 p2 id, {{ pre }} CheckID id ;; p1 >> p2
+  -> {{ pre }} p1 >> p2.
+Proof.
+  unfold corr; intros.
+  eapply H; eauto.
+  destruct (classic (check_cond id m)).
+  - inversion H1; subst.
+    + constructor.
+      apply XCheckOK; eauto.
+    + constructor.
+      apply XCheckOK; eauto.
+    + eapply XRCrashed.
+      apply XCheckOK; eauto.
+      eauto.
+  - assert (Failed=Finished); try discriminate.
+    eapply H; eauto.
+    constructor.
+    apply XCheckFail with (m':=m); eauto.
+Qed.
+
+Theorem corr_drop_check2 : forall pre p1 p2 id, {{ pre }} p1 >> CheckID id ;; p2
+  -> {{ pre }} p1 >> p2.
+Proof.
+  unfold corr; intros.
+  assert (forall m' out, exec_recover m p1 (CheckID id ;; p2) m' out -> out = Finished) by eauto.
+  clear H H0.
+  induction H1; eauto.
+  apply IHexec_recover; clear IHexec_recover.
+  intros.
+  inversion H0; subst; eauto.
+  - eapply H2.
+    eapply XRCrashed; [eassumption|constructor].
+    destruct (classic (check_cond id m')).
+    apply XCheckOK; eauto.
+    apply XCheckFail; eauto.
+  - eapply H2.
+    eapply XRCrashed; [eassumption|].
+    econstructor; [|eauto].
+    destruct (classic (check_cond id m')).
+    apply XCheckOK; eauto.
+    assert (Failed=Finished); try discriminate.
+    eapply H2.
+    eapply XRCrashed; [eassumption|].
+    constructor.
+    apply XCheckFail with (m':=m'); eauto.
+Qed.
+
+Theorem idempotent_nocheck_ok : forall p pre, preserves_precondition pre p
+  -> {{ pre }} p >> p.
+Proof.
+  intros.
+  eapply corr_drop_check2.
+  eapply corr_drop_check1.
+  apply idempotent_ok.
+  eauto.
+Qed.
 
 (* Sketch of how we might prove recover's idempotence *)
+Module RECOVER_SKETCH.
 
-Parameter xrecover : prog -> prog.
-Parameter log_intact : mem -> pred.
-Parameter recovered : mem -> pred.
+  Parameter recover : prog -> prog.
+  Parameter log_intact : mem -> pred.
+  Parameter recovered : mem -> pred.
 
-Theorem recover_base_ok : forall rx id,
-  {{ exists m, log_intact m
-   * [[ guardcond (Done id tt) = log_intact m ]]
-   * [[ {{ recovered m }} rx >> Done id tt ]]
-  }} xrecover rx >> Done id tt.
-Admitted.
+  Axiom recover_base_ok : forall rx id rec,
+    {{ exists m, log_intact m
+     * [[ {{ log_intact m }} rec >> CheckID id ;; rec ]]
+     * [[ {{ recovered m }} rx >> CheckID id ;; rec ]]
+     * [[ check_cond id = log_intact m ]]
+    }} recover rx >> CheckID id ;; rec.
 
-Theorem recover_preserves : forall rx,
-  preserves_precondition
-    (log_intact
-   * [[ {{ recovered }} rx >> Check log_intact ;; Done tt ]])
-    (xrecover rx).
-Proof.
-  intros.
-  eapply corr_to_pp.
-  eapply pimpl_ok. apply recover_base_ok. apply pimpl_refl.
-  repeat ( apply sep_star_lift_l; intros ).
-  unfold lift, pimpl; intros.
-  repeat ( apply sep_star_and2lift; unfold lift; split; eauto ).
-Qed.
+  Theorem recover_preserves_1 : forall rx,
+    preserves_precondition
+      (exists m id rec, log_intact m
+       * [[ check_cond id = log_intact m ]]
+       * [[ {{ log_intact m }} rec >> CheckID id ;; rec ]]
+       * [[ {{ recovered m }} rx >> CheckID id ;; rec ]])%pred
+      (recover rx).
+  Proof.
+    intros.
+    do 3 ( eapply pp_exists; intros ).
+    eapply corr_to_pp.
+    eapply pimpl_ok. apply recover_base_ok. cancel; try eassumption.
+    cancel.
+    cancel.
+  Qed.
 
-Theorem recover_idempotent_ok : forall rx,
-  {{ log_intact
-   * [[ {{ recovered }} rx >> Check log_intact ;; Done tt ]]
-  }} xrecover rx >> xrecover rx.
-Proof.
-  intros.
-  apply idempotent_ok.
-  apply recover_preserves.
-Qed.
+  Theorem recover_preserves_2 : forall rx,
+    preserves_precondition
+      (exists m rec, log_intact m
+       * [[ {{ log_intact m }} rec >> Check (log_intact m) ;; rec ]]
+       * [[ {{ recovered m }} rx >> Check (log_intact m) ;; rec ]])%pred
+      (recover rx).
+  Proof.
+    intros.
+    do 2 ( eapply pp_exists; intros ).
+    unfold Check.
+    eapply corr_to_pp.
+    eapply pimpl_ok. apply recover_base_ok.
+    cancel; try eassumption.
+    rewrite check_id_ok; eauto.
+    cancel.
+    rewrite check_id_ok; cancel.
+  Qed.
+
+  Theorem recover_idempotent_ok_1 : forall rx,
+    {{ exists m rec, log_intact m
+     * [[ {{ log_intact m }} rec >> Check (log_intact m) ;; rec ]]
+     * [[ {{ recovered m }} rx >> Check (log_intact m) ;; rec ]]
+    }} recover rx >> recover rx.
+  Proof.
+    intros.
+    apply idempotent_nocheck_ok.
+    apply recover_preserves_2.
+  Qed.
+
+End RECOVER_SKETCH.
